lambda2Gmu/CanonicalForms.v
@@ -1,5 +1,6 @@
 Require Import Definitions.
 Require Import Infrastructure.
+Require Import Equations.
 Require Import TLC.LibTactics.
 Require Import TLC.LibEnv.
 Require Import TLC.LibLN.
@@ -8,23 +9,25 @@ Require Import TLC.LibLN.
   (* Ht : {Σ, empty}⊢ trm_constructor Tparams Name e1 ∈ T1 ** T2 *)
 Lemma CanonicalConstructorType : forall Σ Δ E Tparams Name Ctor e1 T,
     {Σ, Δ, E} ⊢ trm_constructor Tparams (Name, Ctor) e1 ∈ T ->
+    ~ (contradictory_bounds Σ Δ) ->
     (* TODO can we make Typs more specific? *)
     exists Typs, T = typ_gadt Typs Name.
-  introv Htyp.
+  introv Htyp Hbound.
   inversions Htyp.
   - rewrite rewrite_open_tt_many_gadt.
     eexists.
     f_equal.
-  - admit.
+  - destruct T.
 Admitted.
 
 Lemma CanonicalConstructorTypeGen : forall Σ Δ E Tparams Ctor e1 T,
     {Σ, Δ, E} ⊢ trm_constructor Tparams Ctor e1 ∈ T ->
+    ~ (contradictory_bounds Σ Δ) ->
     (* TODO can we make Typs more specific? *)
     exists Typs Name, T = typ_gadt Typs Name.
   intros.
   destruct Ctor.
-  apply CanonicalConstructorType in H.
+  apply CanonicalConstructorType in H; auto.
   destruct H as [Typs Heq].
   eexists. eexists. eauto.
 Qed.
