lambda2Gmu/Equations.v
@@ -33,24 +33,77 @@ Section SimpleEquationProperties.
     transitivity (subst_tt' U Θ); auto.
   Qed.
 
+  Lemma subst_tt_inside : forall Θ A P T,
+      A \notin substitution_sources Θ ->
+      subst_tt' (subst_tt A P T) Θ
+      =
+      subst_tt A (subst_tt' P Θ) (subst_tt' T Θ).
+  Admitted.
+
+  Lemma teq_axiom : forall Δ T U,
+      List.In (tc_eq (T ≡ U)) Δ ->
+      entails_semantic Σ Δ (T ≡ U).
+    unfold entails_semantic. unfold alpha_equivalent.
+    induction Δ; introv Hin Hmatch.
+    - contradiction.
+    - cbn in Hin.
+      destruct Hin as [Hin | Hin].
+      + subst.
+        inversions Hmatch; easy.
+      + inversions Hmatch; auto.
+        cbn.
+        assert (A \notin substitution_sources Θ0); [admit|idtac].
+        repeat rewrite subst_tt_inside; auto.
+        f_equal.
+        apply IHΔ; auto.
+  Admitted.
+
 End SimpleEquationProperties.
 
+Ltac fold_from_list :=
+  repeat progress match goal with
+  | [ H: context[LibList.fold_right (fun (x : var) (acc : fset var) => \{ x} \u acc) \{} ?L]  |- _ ] =>
+    fold (from_list L) in H
+  | |- context[LibList.fold_right (fun (x : var) (acc : fset var) => \{ x} \u acc) \{} ?L] =>
+    fold (from_list L)
+                  end.
+
+Lemma notin_from_list : forall As (A : var),
+    ~ (List.In A As) ->
+    A \notin from_list As.
+  intros.
+  intro HF.
+  lets [A' [Hin Heq]]: in_from_list HF.
+  subst.
+  auto.
+Qed.
+
 Lemma spawn_unit_subst : forall Σ As,
-    exists Θ, length Θ = length As /\ subst_matches_typctx Σ (tc_vars As) Θ.
-  induction As as [| Ah Ats].
+    DistinctList As ->
+    exists Θ, length Θ = length As /\ subst_matches_typctx Σ (tc_vars As) Θ /\ substitution_sources Θ = from_list As.
+  induction As as [| Ah Ats]; introv ADist.
   - cbn.
     exists (@nil (var * typ)).
-    split~.
+    splits~.
     constructor.
-  - destruct IHAts as [LT [Len Match]].
+  - inversions ADist.
+    destruct IHAts as [LT [Len [Match Src]]]; auto.
     exists ((Ah, typ_unit) :: LT).
-    split.
+    splits.
     + cbn. auto.
-    + constructor.
-      * constructor.
-      * fold (List.map tc_var Ats).
-        fold (tc_vars Ats).
-        trivial.
+    + constructor;
+        fold (List.map tc_var Ats);
+        fold (tc_vars Ats);
+        auto.
+      * rewrite Src.
+        apply~ notin_from_list.
+      * apply notin_dom_tc_vars.
+        apply~ notin_from_list.
+    + cbn.
+      fold_from_list.
+      fold (substitution_sources LT).
+      rewrite Src.
+      trivial.
 Qed.
 
 Lemma only_vars_is_tc_vars : forall Δ,
@@ -68,25 +121,71 @@ Lemma only_vars_is_tc_vars : forall Δ,
     false~ Hin. congruence.
 Qed.
 
-Lemma only_vars_is_never_contradictory : forall Σ Δ,
-    (forall tc, List.In tc Δ -> exists A, tc = tc_var A) ->
-    ~ (contradictory_bounds Σ Δ).
+(* Lemma only_vars_is_never_contradictory : forall Σ Δ, *)
+(*     (forall tc, List.In tc Δ -> exists A, tc = tc_var A) -> *)
+(*     ~ (contradictory_bounds Σ Δ). *)
+(*   intros. *)
+(*   intro HF. *)
+(*   unfold contradictory_bounds in HF. *)
+(*   lets F: HF typ_unit (typ_unit ** typ_unit). *)
+(*   unfold entails_semantic in F. *)
+(*   lets* [As AsEQ]: only_vars_is_tc_vars. subst. *)
+(*   lets [Θ [TLen TMatch]]: spawn_unit_subst Σ As. *)
+(*   assert (Contr: typ_unit = typ_unit ** typ_unit). *)
+(*   - unfold alpha_equivalent in F. *)
+(*     lets F2: F TMatch. *)
+(*     rewrite subst_ttΘ_fresh in F2. *)
+(*     + rewrite~ subst_ttΘ_fresh in F2. *)
+(*       cbn. *)
+(*       rewrite union_empty_r. *)
+(*       rewrite~ inter_empty_r. *)
+(*     + cbn. *)
+(*       rewrite~ inter_empty_r. *)
+(*   - false. *)
+(* Qed. *)
+Lemma adding_var_is_not_contradictory : forall Σ Δ A,
+    ~ (contradictory_bounds Σ Δ) ->
+    ~ (contradictory_bounds Σ (Δ |,| [tc_var A])).
+  introv Hsmal.
+  intro HF.
+  apply Hsmal.
+Admitted.
+
+Lemma adding_vars_is_not_contradictory : forall Σ Δ As,
+    ~ (contradictory_bounds Σ Δ) ->
+    ~ (contradictory_bounds Σ (Δ |,| tc_vars As)).
+  introv Hsmal.
+  induction As.
+  - cbn. clean_empty_Δ. auto.
+  - cbn. fold (tc_vars As).
+  intro HF.
+  apply Hsmal.
+Admitted.
+
+Lemma empty_is_not_contradictory : forall Σ,
+    ~ (contradictory_bounds Σ emptyΔ).
   intros.
   intro HF.
   unfold contradictory_bounds in HF.
-  lets F: HF typ_unit (typ_unit ** typ_unit).
-  unfold entails_semantic in F.
-  lets* [As AsEQ]: only_vars_is_tc_vars. subst.
-  lets [Θ [TLen TMatch]]: spawn_unit_subst Σ As.
-  assert (Contr: typ_unit = typ_unit ** typ_unit).
-  - unfold alpha_equivalent in F.
-    lets F2: F TMatch.
-    rewrite subst_ttΘ_fresh in F2.
-    + rewrite~ subst_ttΘ_fresh in F2.
-      cbn.
-      rewrite union_empty_r.
-      rewrite~ inter_empty_r.
-    + cbn.
-      rewrite~ inter_empty_r.
-  - false.
+  asserts M: (subst_matches_typctx Σ emptyΔ (@nil (var*typ)));
+    try econstructor.
+  lets F: HF typ_unit (typ_unit ** typ_unit) (@nil (var * typ)) M.
+  unfold alpha_equivalent in F.
+  cbn in F.
+  false.
 Qed.
+
+Lemma typing_exfalso : forall Σ Δ E e T1 T2,
+    {Σ, Δ, E} ⊢ e ∈ T1 ->
+    contradictory_bounds Σ Δ ->
+    {Σ, Δ, E} ⊢ e ∈ T2.
+  introv Typ Bounds.
+  apply typing_eq with T1; auto.
+Qed.
+
+(* Lemma generalized_inversion : forall Σ Δ E e T, *)
+(*     {Σ, Δ, E} ⊢ e ∈ T -> *)
+(*     ~ (contradictory_bounds Σ Δ) -> *)
+(*     (exists T', okt Σ Δ E /\ T = typ_unit) \/ True. (* TODO other cases: probably instead I want to add some syntactic separation of equations instead of writing a huge inversion here *) *)
+(*   introv Typ Bounds. *)
+(* Admitted. *)
